theories/All.v
@@ -1,5 +1,5 @@
 From Tableaux Require Export Core.
 
-From Tableaux Require Export ATPCompat.
+From Tableaux Require Export ExtendedSyntax.
 From Tableaux Require Export Reflect.
 
